proofs/lean/extraction/Gcd.lean
@@ -11,64 +11,36 @@ open Std.Tactic
 set_option mvcgen.warning false
 set_option linter.unusedVariables false
 
-class Gcd.Gcd (Self : Type) where
-  gcd : (Self -> Self -> Result Self)
-  gcd_binary : (Self -> Self -> Result Self)
-  gcd_euclid : (Self -> Self -> Result Self)
-
-def Rust_primitives.Hax.Machine_int.bitor {α β γ} [HOr α β γ] (x:α) (y:β) : Result γ := pure (HOr.hOr x y)
-
-def Core.Num.Impl_6.trailing_zeros : u8 -> Result u32 := sorry
-instance : HaxShiftRight u8 u32 := sorry
-open Rust_primitives
-
 def Hax_lib.Int.Int : Type := _root_.Int
-def Hax.Int.from_machine : u32 → Hax_lib.Int.Int := sorry
-def Hax.while_loop_cf {State: Type}
-  (inv: State → Result Bool)
+def Rust_primitives.Hax.while_loop {State: Type}
   (cond: State → Result Bool)
-  (termination : State -> Result Hax_lib.Int.Int)
-  (init : State)
-  (body : State -> Result (Core.Ops.Control_flow.ControlFlow (Hax.Tuple2 Hax.Tuple0 State) State))
-  : Result State := sorry
-
-def Hax.while_loop {State: Type}
   (inv: State → Result Bool)
-  (cond: State → Result Bool)
   (termination : State -> Result Hax_lib.Int.Int)
   (init : State)
   (body : State -> Result State)
   : Result State := sorry
-def Hax.Machine_int.shl : u8 -> u32 -> Result u8 := sorry
+def Rust_primitives.Hax.Int.from_machine (x : u8) : Hax_lib.Int.Int := Int.ofNat x.toNat
 
 -- Const euclid GCD implementation for `u8`.
 def Gcd.euclid_u8 (a : u8) (b : u8) : Result u8 := do
   let ⟨a, b⟩ ←
-    if (← (Hax.Machine_int.gt a b)) then
-      (pure (Hax.Tuple2.mk a b))
+    if (← (Rust_primitives.Hax.Machine_int.gt a b)) then
+      (pure (Rust_primitives.Hax.Tuple2.mk a b))
     else
-      (pure (Hax.Tuple2.mk b a));
+      (pure (Rust_primitives.Hax.Tuple2.mk b a));
   let ⟨a, b⟩ ←
-    (Hax.while_loop
+    (Rust_primitives.Hax.while_loop
       (fun ⟨a, b⟩ => (do
-        (Hax.Machine_int.ne b (0 : u8)) : Result Bool))
+        (Rust_primitives.Hax.Machine_int.ne b (0 : u8)) : Result Bool))
       (fun ⟨a, b⟩ => (do (pure true) : Result Bool))
       (fun ⟨a, b⟩ => (do
-        (Hax.Int.from_machine (0 : u32)) : Result
-        Hax_lib.Int.Int))
-      (Hax.Tuple2.mk a b)
+        (Rust_primitives.Hax.Int.from_machine b) : Result Hax_lib.Int.Int))
+      (Rust_primitives.Hax.Tuple2.mk a b)
       (fun ⟨a, b⟩ => (do
         let temp : u8 := a;
         let a : u8 := b;
         let b : u8 := temp;
         let b : u8 ← (b %? a);
-        (pure (Hax.Tuple2.mk a b)) : Result
-        (Hax.Tuple2 u8 u8))));
+        (pure (Rust_primitives.Hax.Tuple2.mk a b)) : Result
+        (Rust_primitives.Hax.Tuple2 u8 u8))));
   (pure a)
-
-theorem Gcd.euclid_u8.spec (a:u8) (b:u8) :
-  ⦃ ⌜ True ⌝ ⦄
-  (euclid_u8 a b)
-  ⦃ ⇓ r => ⌜ True ⌝ ⦄
-  := by
-  mvcgen [euclid_u8]
