proofs/lean/extraction/Verif.lean
@@ -1,0 +1,60 @@
+import extraction.Gcd
+open Std.Do
+open Std.Tactic
+
+@[spec]
+theorem Rust_primitives.Hax.while_loop.spec {State: Type}
+  (cond: State → Result Bool)
+  (inv: State → Result Bool)
+  (termination : State -> Result Int)
+  (init : State)
+  (body : State -> Result State) :
+  -- inv init = pure true →
+  -- (∀ state,
+  --   inv state = pure true →
+  --   cond state = pure true →
+  --   ⦃ ⌜ True ⌝ ⦄
+  --   do
+  --     let state ← body state
+  --     inv state
+  --   ⦃ ⇓ isInvTrue => ⌜ isInvTrue ⌝ ⦄) →
+  (∀ state,
+    ⦃ ⌜ True ⌝ ⦄
+    do
+      if ← cond state then
+        let state' ← body state
+        let m ← termination state
+        let m' ← termination state'
+        pure (some (m, m'))
+      else
+        pure none
+    ⦃ ⇓ r => ⌜ match r with
+      | none => True
+      | some (m, m') => (0 ≤ m' ∧ m' < m) ⌝ ⦄) →
+  ⦃ ⌜ True ⌝ ⦄
+  Rust_primitives.Hax.while_loop cond inv termination init body
+  ⦃ ⇓ r => ⌜ True ⌝ ⦄ := by sorry
+
+
+@[spec]
+theorem Hax.rem (a:u8) (b:u8) (hb :b ≠ 0) :
+  ⦃ ⌜ True ⌝ ⦄
+  (a %? b)
+  ⦃ ⇓ r => ⌜ r < b ⌝ ⦄
+  := sorry
+
+
+theorem Gcd.euclid_u8.spec (a:u8) (b:u8) :
+  ⦃ ⌜ True ⌝ ⦄
+  (euclid_u8 a b)
+  ⦃ ⇓ r => ⌜ True ⌝ ⦄
+  := by
+  mvcgen (stepLimit := none) [euclid_u8]
+  · grind
+  · constructor
+    apply Int.zero_le_ofNat
+    exact Int.lt_of_toNat_lt (by assumption)
+  · grind
+  · constructor
+    apply Int.zero_le_ofNat
+    exact Int.lt_of_toNat_lt (by assumption)
